core/Utils.v
@@ -2,13 +2,32 @@ From Ssara.Core Require Import Syntax.
 From Ssara.Core Require Import Vm.
 From Stdlib Require Import ZArith.
 From Stdlib Require Import ListSet.
+From Stdlib Require Import Lists.List.
+
+From Ssara.Core Require Import RegNatInstance.
+Existing Instance reg_instance.
 
 (* Set of registers *)
-Definition reg_eq_dec : forall r r' : reg, {r = r'} + {r <> r'} := Nat.eq_dec.
+Definition reg_eq_dec : forall r r' : reg, {r = r'} + {r <> r'} := reg_eq_dec.
 Definition regs_union := set_union reg_eq_dec.
 Definition regs_diff := set_diff reg_eq_dec.
 Definition regs_add := set_add reg_eq_dec.
 Definition regs_remove := set_remove reg_eq_dec.
+
+(* Lemma regs_remove_absence :
+  forall (r : reg) (regs : set reg),
+    In r regs -> length (regs_remove r regs) < length regs
+.
+Proof.
+  induction regs as [| x xs IH]; simpl; intros Hin.
+  - inversion Hin.
+  - destruct reg_eq_dec as [Heq | Hneq].
+    + subst.
+      apply Nat.lt_succ_diag_r.
+    + simpl.
+      apply -> Nat.succ_lt_mono.
+      assert (In r xs) as Hin_t by (destruct Hin; [contradiction | assumption]). *)
+
 Definition regs_mem := set_mem reg_eq_dec.
 
 (* Set of labels *)
