core/RegPregInstance.v
@@ -1,0 +1,43 @@
+From Stdlib Require Import PeanoNat.
+From Ssara.Core Require Import Syntax.
+
+Inductive preg : Type :=
+  | RAX
+  | RBX
+  | RCX
+  | RDX
+  | RSI
+  | RDI
+  | RSP
+  | RBP
+.
+
+Definition preg_eqb (p : preg) (p' : preg) : bool :=
+  match p, p' with
+  | RAX, RAX => true
+  | RBX, RBX => true
+  | RCX, RCX => true
+  | RDX, RDX => true
+  | RSI, RSI => true
+  | RDI, RDI => true
+  | RSP, RSP => true
+  | RBP, RBP => true
+  | _, _ => false
+  end
+.
+
+Lemma preg_eqb_eq : forall r r', preg_eqb r r' = true <-> r = r'.
+Proof.
+  destruct r, r'; simpl; split; try congruence; intros; reflexivity.
+Qed.
+
+Lemma preg_eq_dec : forall r r' : preg, {r = r'} + {r <> r'}.
+Proof.
+  decide equality.
+Qed.
+
+Instance reg_instance : RegClass := {|
+  reg := preg;
+  reg_eqb := preg_eqb;
+  reg_eq_dec := preg_eq_dec;
+|}.
